\begin{table}[ht]
  \begin{center}
    \begin{tabular*}{\textwidth}{l p{\textwidth}}
      \hline \\
      \hspace{0.5cm} $[\mbox{LIST}_{\mbox{ACCESS-1}}]$ & \infrule{env_{T},
      env_{C}, env_{V} \vdash \lag E\; \rag \ra v_2  \qquad env_{T}, env_{C},
      env_{V} \vdash \lag L \rag \ra v_3}
      {env_{T}, env_{C}, env_{V} \vdash \lag E\; L \rag \ra v_1} \\
       & where $v_2 = \left(l_1, elem_1\right)$ \\
       & and $v_3 = (l_2,elem_2)$ \\
       & and $l_2 = 1$ \\
       & and $i = elem_2\; 0$ \vspace{0.1cm} \\
       & and $v_1 = \left\{
	 \begin{array}{l l}
           elem_1\; i         & \quad \text{if $i \geq 0$}\\
           elem_1\; (l_1 + i) & \quad \text{if $i < 0$}
	 \end{array} \right.$ \\
	 
      \hspace{0.5cm} $[\mbox{LIST}_{\mbox{ACCESS-2}}]$ & \infrule{env_{T},
      env_{C}, env_{V} \vdash \lag E \rag \ra v_2  \qquad env_{T}, env_{C},
      env_{V} \vdash \lag L \rag \ra v_3}
      {env_{T}, env_{C}, env_{V} \vdash \lag E\; L \rag \ra v_1} \\
       & where $v_2 = \left(l_1, elem_1\right)$ \\
       & and $v_3 = (l_2,elem_2)$ \\
       & and $l_2 = 2$ \vspace{0.1cm} \\
       & and $i = \left\{
	 \begin{array}{l l}
           elem_2\; 0         & \quad \text{if $elem_2\; 0 \geq 0$}\\
           l_1 + elem_2\; 0   & \quad \text{if $elem_2\; 0 < 0$}
	 \end{array} \right.$ \vspace{0.1cm} \\
       & and $j = \left\{
	 \begin{array}{l l}
           elem_2\; 1         & \quad \text{if $elem_2\; 1 \geq 0$}\\
           l_1 + elem_2\; 1   & \quad \text{if $elem_2\; 1 < 0$}
	 \end{array} \right.$ \vspace{0.1cm} \\
       & and $elem_3\; z = \left\{
	 \begin{array}{l l}
           elem_1\; i+1       & \quad \text{if $z = 0$}\\
	   \hspace{1cm} \vdots &   \\
           elem_1\; i+n-1     & \quad \text{if $z = n-1$}
	 \end{array} \right.$ \vspace{0.1cm} \\
       & and $v_1 = (n=j-i+1,\; elem_3)$ \\
       & \\
       \hline
    \end{tabular*}
    \capt{Transition rules for accessing lists.}
    \label{semantic:lists}
  \end{center}
\end{table}

